theories/transform/Transform.v
@@ -25,23 +25,6 @@ Variable nq: nat.
 Definition Qbit_index_valid (qbit: nat): Prop :=
   nq > qbit.
 
-Lemma Transform_I_Branch:
-  forall (b: Branch nq) (qbit: nat),
-  b = Execute_rotate_instr_branch nq 0 0 0 qbit b.
-Proof.
-  intros b qbit.
-  unfold Execute_rotate_instr_branch.
-  destruct b eqn:Hb.
-  simpl.
-  f_equal.
-  rewrite Gate_P_matrix_0_eye.
-  rewrite mat_single_eye.
-  unfold den_uop.
-  rewrite mat_eye_conjtrans.
-  rewrite mat_mul_eye_l, mat_mul_eye_r.
-  reflexivity.
-Qed.
-
 Lemma Transform_I: forall (qbit: nat),
   Instruction_equiv nq
   (Gate_I qbit)
@@ -51,19 +34,20 @@ Proof.
   unfold Instruction_equiv, ProgramState_equiv.
   intros ps Hinv.
   unfold PositiveMap.Equal.
-  intros cstate.
-  simpl.
-  destruct (PositiveMap.find cstate ps) eqn:Hfind.
-  - rewrite <- PFacts.find_mapsto_iff.
-    rewrite <- PFacts.find_mapsto_iff in Hfind.
-    unfold Execute_rotate_instr.
-    rewrite (Transform_I_Branch b qbit).
-    apply PositiveMap.map_1.
-    apply Hfind.
-  - unfold Execute_rotate_instr.
-    rewrite PFacts.map_o.
-    rewrite Hfind.
-    simpl. reflexivity.
+  intros cstate. simpl.
+  unfold Execute_rotate_instr.
+  rewrite PFacts.map_o.
+  destruct (PositiveMap.find cstate ps); simpl.
+  - f_equal.
+    unfold Execute_rotate_instr_branch.
+    destruct b; simpl; f_equal.
+    rewrite Gate_P_matrix_0_eye.
+    rewrite mat_single_eye.
+    unfold den_uop.
+    rewrite mat_eye_conjtrans.
+    rewrite mat_mul_eye_l, mat_mul_eye_r.
+    reflexivity.
+  - reflexivity.
 Qed.
 
 Lemma Transform_den_uop_involutive:
@@ -72,31 +56,12 @@ Lemma Transform_den_uop_involutive:
   den_uop A (den_uop A Q) = Q.
 Proof.
   intros A Q Hu HH.
+  rewrite den_uop_den_uop.
+  rewrite <- HH at 2.
+  rewrite (proj2 Hu).
   unfold den_uop.
-  rewrite mat_mul_assoc, mat_mul_assoc.
-  rewrite <- HH at 2. rewrite HH at 2.
-  rewrite (proj2 Hu), mat_mul_eye_l.
-  rewrite <- mat_mul_assoc.
-  rewrite (proj2 Hu), mat_mul_eye_r.
+  rewrite mat_mul_eye_l, mat_eye_conjtrans, mat_mul_eye_r.
   reflexivity.
-Qed.
-
-Lemma Transform_X_X_Branch:
-  forall (b: Branch nq) (qbit: nat),
-  Qbit_index_valid qbit ->
-  b = Execute_rotate_instr_branch nq PI 0 PI qbit (Execute_rotate_instr_branch nq PI 0 PI qbit b).
-Proof.
-  intros b qbit H.
-  unfold Execute_rotate_instr_branch.
-  destruct b eqn:Hb.
-  simpl.
-  f_equal.
-  rewrite Gate_X_matrix_gphase.
-  rewrite (Gate_matrix_den_uop_gphase _ _ H), (Gate_matrix_den_uop_gphase _ _ H).
-  rewrite Transform_den_uop_involutive.
-  - reflexivity.
-  - apply mat_single_unitary. apply Gate_X_matrix_unitary.
-  - apply mat_single_Hermitian. apply Gate_X_matrix_Hermitian.
 Qed.
 
 Lemma Transform_X_X: forall (qbit: nat),
@@ -110,36 +75,17 @@ Proof.
   intros H ps Hinv.
   unfold PositiveMap.Equal.
   intros cstate. simpl.
-  destruct (PositiveMap.find cstate ps) eqn:Hfind.
-  - rewrite <- PFacts.find_mapsto_iff.
-    rewrite <- PFacts.find_mapsto_iff in Hfind.
-    unfold Execute_rotate_instr.
-    rewrite (Transform_X_X_Branch _ _ H).
-    apply PositiveMap.map_1.
-    apply PositiveMap.map_1.
-    apply Hfind.
-  - unfold Execute_rotate_instr.
-    rewrite PFacts.map_o, PFacts.map_o.
-    rewrite Hfind.
-    simpl. reflexivity.
-Qed.
-
-Lemma Transform_Y_Y_Branch:
-  forall (b: Branch nq) (qbit: nat),
-  Qbit_index_valid qbit ->
-  b = Execute_rotate_instr_branch nq PI PI2 PI2 qbit (Execute_rotate_instr_branch nq PI PI2 PI2 qbit b).
-Proof.
-  intros b qbit H.
-  unfold Execute_rotate_instr_branch.
-  destruct b eqn:Hb.
-  simpl.
-  f_equal.
-  rewrite Gate_Y_matrix_gphase.
-  rewrite (Gate_matrix_den_uop_gphase _ _ H), (Gate_matrix_den_uop_gphase _ _ H).
-  rewrite Transform_den_uop_involutive.
+  unfold Execute_rotate_instr.
+  repeat rewrite PFacts.map_o.
+  destruct (PositiveMap.find cstate ps); simpl.
+  - f_equal.
+    unfold Execute_rotate_instr_branch.
+    destruct b; simpl; f_equal.
+    rewrite Gate_X_matrix_gphase, (Gate_matrix_den_uop_gphase _ _ H), (Gate_matrix_den_uop_gphase _ _ H).
+    apply Transform_den_uop_involutive.
+    + apply mat_single_unitary. apply Gate_X_matrix_unitary.
+    + apply mat_single_Hermitian. apply Gate_X_matrix_Hermitian.
   - reflexivity.
-  - apply mat_single_unitary. apply Gate_Y_matrix_unitary.
-  - apply mat_single_Hermitian. apply Gate_Y_matrix_Hermitian.
 Qed.
 
 Lemma Transform_Y_Y: forall (qbit: nat),
@@ -153,36 +99,17 @@ Proof.
   intros H ps Hinv.
   unfold PositiveMap.Equal.
   intros cstate. simpl.
-  destruct (PositiveMap.find cstate ps) eqn:Hfind.
-  - rewrite <- PFacts.find_mapsto_iff.
-    rewrite <- PFacts.find_mapsto_iff in Hfind.
-    unfold Execute_rotate_instr.
-    rewrite (Transform_Y_Y_Branch _ _ H).
-    apply PositiveMap.map_1.
-    apply PositiveMap.map_1.
-    apply Hfind.
-  - unfold Execute_rotate_instr.
-    rewrite PFacts.map_o, PFacts.map_o.
-    rewrite Hfind.
-    simpl. reflexivity.
-Qed.
-
-Lemma Transform_Z_Z_Branch:
-  forall (b: Branch nq) (qbit: nat),
-  Qbit_index_valid qbit ->
-  b = Execute_rotate_instr_branch nq 0 0 PI qbit (Execute_rotate_instr_branch nq 0 0 PI qbit b).
-Proof.
-  intros b qbit H.
-  unfold Execute_rotate_instr_branch.
-  destruct b eqn:Hb.
-  simpl.
-  f_equal.
-  rewrite Gate_Z_matrix_gphase.
-  rewrite (Gate_matrix_den_uop_gphase _ _ H), (Gate_matrix_den_uop_gphase _ _ H).
-  rewrite Transform_den_uop_involutive.
+  unfold Execute_rotate_instr.
+  repeat rewrite PFacts.map_o.
+  destruct (PositiveMap.find cstate ps); simpl.
+  - f_equal.
+    unfold Execute_rotate_instr_branch.
+    destruct b; simpl; f_equal.
+    rewrite Gate_Y_matrix_gphase, (Gate_matrix_den_uop_gphase _ _ H), (Gate_matrix_den_uop_gphase _ _ H).
+    apply Transform_den_uop_involutive.
+    + apply mat_single_unitary. apply Gate_Y_matrix_unitary.
+    + apply mat_single_Hermitian. apply Gate_Y_matrix_Hermitian.
   - reflexivity.
-  - apply mat_single_unitary. apply Gate_Z_matrix_unitary.
-  - apply mat_single_Hermitian. apply Gate_Z_matrix_Hermitian.
 Qed.
 
 Lemma Transform_Z_Z: forall (qbit: nat),
@@ -196,18 +123,41 @@ Proof.
   intros H ps Hinv.
   unfold PositiveMap.Equal.
   intros cstate. simpl.
-  destruct (PositiveMap.find cstate ps) eqn:Hfind.
-  - rewrite <- PFacts.find_mapsto_iff.
-    rewrite <- PFacts.find_mapsto_iff in Hfind.
-    unfold Execute_rotate_instr.
-    rewrite (Transform_Z_Z_Branch _ _ H).
-    apply PositiveMap.map_1.
-    apply PositiveMap.map_1.
-    apply Hfind.
-  - unfold Execute_rotate_instr.
-    rewrite PFacts.map_o, PFacts.map_o.
-    rewrite Hfind.
-    simpl. reflexivity.
+  unfold Execute_rotate_instr.
+  repeat rewrite PFacts.map_o.
+  destruct (PositiveMap.find cstate ps); simpl.
+  - f_equal.
+    unfold Execute_rotate_instr_branch.
+    destruct b; simpl; f_equal.
+    rewrite Gate_Z_matrix_gphase, (Gate_matrix_den_uop_gphase _ _ H), (Gate_matrix_den_uop_gphase _ _ H).
+    apply Transform_den_uop_involutive.
+    + apply mat_single_unitary. apply Gate_Z_matrix_unitary.
+    + apply mat_single_Hermitian. apply Gate_Z_matrix_Hermitian.
+  - reflexivity.
+Qed.
+
+Lemma Transform_H_H: forall (qbit: nat),
+  Qbit_index_valid qbit ->
+  Instruction_equiv nq
+  (SeqInstr (Gate_H qbit) (Gate_H qbit))
+  NopInstr.
+Proof.
+  intros qbit.
+  unfold Instruction_equiv, ProgramState_equiv.
+  intros H ps Hinv.
+  unfold PositiveMap.Equal.
+  intros cstate. simpl.
+  unfold Execute_rotate_instr.
+  repeat rewrite PFacts.map_o.
+  destruct (PositiveMap.find cstate ps); simpl.
+  - f_equal.
+    unfold Execute_rotate_instr_branch.
+    destruct b; simpl; f_equal.
+    rewrite Gate_H_matrix_gphase, (Gate_matrix_den_uop_gphase _ _ H), (Gate_matrix_den_uop_gphase _ _ H).
+    apply Transform_den_uop_involutive.
+    + apply mat_single_unitary. apply Gate_H_matrix_unitary.
+    + apply mat_single_Hermitian. apply Gate_H_matrix_Hermitian.
+  - reflexivity.
 Qed.
 
 Lemma Transform_P_P: forall (qbit: nat) (l1 l2: R),
@@ -221,7 +171,143 @@ Proof.
   intros ps Hinv.
   unfold PositiveMap.Equal.
   intros cstate. simpl.
-  destruct (PositiveMap.find cstate ps) eqn:Hfind.
-Admitted.
+  unfold Execute_rotate_instr.
+  repeat rewrite PFacts.map_o.
+  destruct (PositiveMap.find cstate ps); simpl.
+  - f_equal.
+    unfold Execute_rotate_instr_branch.
+    simpl; f_equal.
+    rewrite den_uop_den_uop. f_equal.
+    rewrite mat_single_factorized. f_equal.
+    rewrite (Rplus_comm l1 l2).
+    apply Gate_P_matrix_mul.
+  - reflexivity.
+Qed.
+
+Lemma Transform_P_periodic: forall (qbit: nat) (l: R),
+  Qbit_index_valid qbit ->
+  Instruction_equiv nq
+  (Gate_P l qbit)
+  (Gate_P (l + 2*PI) qbit).
+Proof.
+  intros qbit l H.
+  unfold Instruction_equiv, ProgramState_equiv.
+  intros ps Hinv.
+  unfold PositiveMap.Equal.
+  intros cstate. simpl.
+  unfold Execute_rotate_instr.
+  repeat rewrite PFacts.map_o.
+  destruct (PositiveMap.find cstate ps); simpl.
+  - f_equal.
+    unfold Execute_rotate_instr_branch.
+    f_equal.
+    rewrite Gate_P_matrix_periodic.
+    rewrite (Gate_matrix_den_uop_gphase _ _ H).
+    reflexivity.
+  - reflexivity. 
+Qed.
+
+Corollary Transform_S_S: forall (qbit: nat),
+  Qbit_index_valid qbit ->
+  Instruction_equiv nq
+  (SeqInstr (Gate_S qbit) (Gate_S qbit))
+  (Gate_Z qbit).
+Proof.
+  intros qbit H.
+  unfold Gate_S, Gate_Z.
+  replace PI with (PI2 + PI2)%R by (unfold PI; field).
+  apply (Transform_P_P qbit _ _ H).
+Qed.
+
+Corollary Transform_S_Sdg: forall (qbit: nat),
+  Qbit_index_valid qbit ->
+  Instruction_equiv nq
+  (SeqInstr (Gate_S qbit) (Gate_Sdg qbit))
+  (Gate_I qbit).
+Proof.
+  intros qbit H.
+  unfold Gate_S, Gate_Sdg, Gate_I.
+  replace 0%R with (PI2 + (- PI2))%R by field.
+  apply (Transform_P_P qbit _ _ H).
+Qed.
+
+Corollary Transform_Sdg_S: forall (qbit: nat),
+  Qbit_index_valid qbit ->
+  Instruction_equiv nq
+  (SeqInstr (Gate_Sdg qbit) (Gate_S qbit))
+  (Gate_I qbit).
+Proof.
+  intros qbit H.
+  unfold Gate_S, Gate_Sdg, Gate_I.
+  replace 0%R with ((- PI2) + PI2)%R by field.
+  apply (Transform_P_P qbit _ _ H).
+Qed.
+
+Corollary Transform_Sdg_Sdg: forall (qbit: nat),
+  Qbit_index_valid qbit ->
+  Instruction_equiv nq
+  (SeqInstr (Gate_Sdg qbit) (Gate_Sdg qbit))
+  (Gate_Z qbit).
+Proof.
+  intros qbit H.
+  unfold Gate_S, Gate_Sdg, Gate_Z.
+  apply Instruction_equiv_equivalence with (y := Gate_P ((-PI2) + (-PI2)) qbit).
+  - apply (Transform_P_P qbit _ _ H).
+  - replace PI with ((-PI) + 2*PI)%R by field.
+    replace ((- PI2) + (-PI2))%R with (-PI)%R by (unfold PI; field).
+    apply (Transform_P_periodic qbit _ H).
+Qed.
+
+Lemma Transform_X_Y: forall (qbit: nat),
+  Qbit_index_valid qbit ->
+  Instruction_equiv nq
+  (SeqInstr (Gate_X qbit) (Gate_Y qbit))
+  (Gate_Z qbit).
+Proof.
+  intros qbit.
+  unfold Instruction_equiv, ProgramState_equiv.
+  intros H ps Hinv.
+  unfold PositiveMap.Equal.
+  intros cstate. simpl.
+  unfold Execute_rotate_instr.
+  repeat rewrite PFacts.map_o.
+  destruct (PositiveMap.find cstate ps); simpl.
+  - f_equal.
+    unfold Execute_rotate_instr_branch.
+    destruct b; simpl; f_equal.
+    rewrite den_uop_den_uop, mat_single_factorized.
+    rewrite Gate_X_matrix_gphase, Gate_Y_matrix_gphase, Gate_Z_matrix_gphase.
+    rewrite <- mat_scale_mul_comm, mat_scale_mul_assoc, mat_scale_mul_assoc.
+    rewrite Gate_matrix_Y_X__eq__Z.
+    repeat rewrite (Gate_matrix_den_uop_gphase _ _ H).
+    reflexivity.
+  - reflexivity.
+Qed.
+
+Lemma Transform_Y_X: forall (qbit: nat),
+  Qbit_index_valid qbit ->
+  Instruction_equiv nq
+  (SeqInstr (Gate_Y qbit) (Gate_X qbit))
+  (Gate_Z qbit).
+Proof.
+  intros qbit.
+  unfold Instruction_equiv, ProgramState_equiv.
+  intros H ps Hinv.
+  unfold PositiveMap.Equal.
+  intros cstate. simpl.
+  unfold Execute_rotate_instr.
+  repeat rewrite PFacts.map_o.
+  destruct (PositiveMap.find cstate ps); simpl.
+  - f_equal.
+    unfold Execute_rotate_instr_branch.
+    destruct b; simpl; f_equal.
+    rewrite den_uop_den_uop, mat_single_factorized.
+    rewrite Gate_X_matrix_gphase, Gate_Y_matrix_gphase, Gate_Z_matrix_gphase.
+    rewrite <- mat_scale_mul_comm, mat_scale_mul_assoc, mat_scale_mul_assoc.
+    rewrite Gate_matrix_X_Y__eq__Z.
+    repeat rewrite (Gate_matrix_den_uop_gphase _ _ H).
+    reflexivity.
+  - reflexivity.
+Qed.
 
 End Transform.
